theories/iris/examples/segment/example02robust.v
@@ -849,7 +849,7 @@ Section Example02Host.
     iDestruct ("Hrestoreglobs" with "Hgdumm") as "Hadvglobs". 
 
     iApply weakestpre.fupd_wp.
-    iMod (interp_instance_alloc [] ⊤ with "[] [] [] [] [] [Hadvfuncs Hadvtabs Hadvmems Hadvglobs]") as "(#Hi & (#Hiresf & _ & _ & #Hiresg) & _)".
+    iMod (interp_instance_alloc [] ⊤ with "[] [] [] [] [] [Hadvfuncs Hadvtabs Hadvmems Hadvglobs]") as "(#Hi & _ & (#Hiresf & _ & _ & #Hiresg) & _)".
     apply Hadvtype'.
     repeat split => //=.
     by rewrite Heqadvm.
